pushing updates to VerifySKC in prep for meeting

intermediate/Veritas.Intermediate.VerifySKC.fst
@@ -201,19 +201,6 @@ let vevictbm (s:slot_id) (s':slot_id) (t:timestamp) (vs:vtls {Valid? vs}): vtls 
             let st_upd = update_store st s' (MVal v'_upd) in
             vevictb s t (update_thread_store vs st_upd)
 
-// TODO: what should the initial size be?
-let store_size = 65536 // 2 ^ 16
-let empty_store:vstore = { data=Seq.create store_size None; is_map=true }
-
-(* Initialize verifier state *)
-let init_thread_state (id:thread_id): vtls = 
-  let vs = Valid id empty_store (MkTimestamp 0 0) empty_hash_value empty_hash_value in  
-  if id = 0 then
-    let st0 = thread_store vs in
-    let st0_upd = add_to_store st0 0 Root (init_value Root) Spec.MAdd in
-    update_thread_store vs st0_upd    
-  else vs
-
 let lemma_store_contains (st:vstore) (st':Spec.vstore) (s:slot_id) (k:key)
   : Lemma (requires (store_rel st st' /\ slot_key_equiv st s k))
           (ensures (store_contains st s = Spec.store_contains st' k))
@@ -244,6 +231,11 @@ let lemma_vget_simulates_spec
     lemma_store_contains st st' s k;
     lemma_stored_value st st' s k
 
+let lemma_vget_has_failed (vs:vtls{Valid? vs}) (s:slot_id) (v:data_value)
+  : Lemma (requires (not (thread_store_is_map vs)))
+          (ensures (has_failed (vget s v vs)))
+  = admit()
+
 let lemma_vput_simulates_spec 
       (vs:vtls{Valid? vs}) 
       (vs':Spec.vtls{Spec.Valid? vs'}) 
@@ -256,6 +248,11 @@ let lemma_vput_simulates_spec
     let st' = Spec.thread_store vs' in
     lemma_store_contains st st' s k;
     lemma_update_store st st' s k v
+
+let lemma_vput_has_failed (vs:vtls{Valid? vs}) (s:slot_id) (v:data_value)
+  : Lemma (requires (not (thread_store_is_map vs)))
+          (ensures (has_failed (vput s v vs)))
+  = admit()
 
 let lemma_vaddm_simulates_spec 
       (vs:vtls{Valid? vs}) 
@@ -271,6 +268,11 @@ let lemma_vaddm_simulates_spec
     // ...
     admit()
 
+let lemma_vaddm_has_failed (vs:vtls{Valid? vs}) (s s':slot_id) (r:record)
+  : Lemma (requires (not (thread_store_is_map vs)))
+          (ensures (has_failed (vaddm s r s' vs)))
+  = admit()
+
 let lemma_vevictm_simulates_spec 
       (vs:vtls{Valid? vs}) 
       (vs':Spec.vtls{Spec.Valid? vs'}) 
@@ -279,6 +281,11 @@ let lemma_vevictm_simulates_spec
       (k':merkle_key)  
   : Lemma (requires (vtls_rel vs vs' /\ slot_key_rel vs s k /\ slot_key_rel vs s' k'))
           (ensures (vtls_rel (vevictm s s' vs) (Spec.vevictm k k' vs'))) 
+  = admit()
+
+let lemma_vevictm_has_failed (vs:vtls{Valid? vs}) (s s':slot_id)
+  : Lemma (requires (not (thread_store_is_map vs)))
+          (ensures (has_failed (vevictm s s' vs)))
   = admit()
 
 let lemma_vaddb_simulates_spec 
@@ -292,6 +299,11 @@ let lemma_vaddb_simulates_spec
           (ensures (vtls_rel (vaddb s r t j vs) (Spec.vaddb r t j vs'))) 
   = admit()
 
+let lemma_vaddb_has_failed (vs:vtls{Valid? vs}) (s:slot_id) (r:record) (t:timestamp) (j:thread_id)
+  : Lemma (requires (not (thread_store_is_map vs)))
+          (ensures (has_failed (vaddb s r t j vs)))
+  = admit()
+
 let lemma_vevictb_simulates_spec 
       (vs:vtls{Valid? vs}) 
       (vs':Spec.vtls{Spec.Valid? vs'}) 
@@ -300,6 +312,11 @@ let lemma_vevictb_simulates_spec
       (t:timestamp)
   : Lemma (requires (vtls_rel vs vs' /\ slot_key_rel vs s k))
           (ensures (vtls_rel (vevictb s t vs) (Spec.vevictb k t vs'))) 
+  = admit()
+
+let lemma_vevictb_has_failed (vs:vtls{Valid? vs}) (s:slot_id) (t:timestamp)
+  : Lemma (requires (not (thread_store_is_map vs)))
+          (ensures (has_failed (vevictb s t vs)))
   = admit()
 
 let lemma_vevictbm_simulates_spec 
@@ -313,22 +330,88 @@ let lemma_vevictbm_simulates_spec
           (ensures (vtls_rel (vevictbm s s' t vs) (Spec.vevictbm k k' t vs'))) 
   = admit()
 
-(*
+let lemma_vevictbm_has_failed (vs:vtls{Valid? vs}) (s s':slot_id) (t:timestamp)
+  : Lemma (requires (not (thread_store_is_map vs)))
+          (ensures (has_failed (vevictbm s s' t vs)))
+  = admit()
+
+// TODO: what should the initial size be?
+let store_size = 65536 // 2 ^ 16
+let empty_store:vstore = { data=Seq.create store_size None; is_map=true }
+
+(* Initialize verifier state *)
+let init_thread_state (id:thread_id): vtls = 
+  let vs = Valid id empty_store (MkTimestamp 0 0) empty_hash_value empty_hash_value in  
+  if id = 0 then
+    let st0 = thread_store vs in
+    let st0_upd = add_to_store st0 0 Root (init_value Root) Spec.MAdd in
+    update_thread_store vs st0_upd    
+  else vs
+
+let init_thread_state_valid (id:thread_id)
+  : Lemma (Valid? (init_thread_state id))
+  = admit()
+
+let lemma_init_thread_state_rel (id:thread_id)
+  : Lemma (vtls_rel (init_thread_state id) (Spec.init_thread_state id))
+  = admit()
+
+let lemma_t_verify_step_simulates_spec (vs:vtls) (vs':Spec.vtls) (e:logSK_entry) (e':logK_entry)
+  : Lemma (requires (vtls_rel vs vs' /\ (has_failed vs \/ log_entry_rel vs e e')))
+          (ensures (vtls_rel (t_verify_step vs e) (Spec.t_verify_step vs' e')))
+  = if Valid? vs
+    then if thread_store_is_map vs
+    then
+      match e, e' with
+      | Get_SK s _ v, Spec.Get k v' -> 
+          lemma_vget_simulates_spec vs vs' s k v
+      | Put_SK s _ v, Spec.Put k v' ->  
+          lemma_vput_simulates_spec vs vs' s k v
+      | AddM_SK s r s' _, Spec.AddM r' k' ->  
+          lemma_vaddm_simulates_spec vs vs' s s' r k'
+      | EvictM_SK s _ s' _, Spec.EvictM k k' ->  
+          lemma_vevictm_simulates_spec vs vs' s s' k k'
+      | AddB_SK s r t j, Spec.AddB r' t' j' ->  
+          lemma_vaddb_simulates_spec vs vs' s r t j
+      | EvictB_SK s _ t, Spec.EvictB k t' ->  
+          lemma_vevictb_simulates_spec vs vs' s k t
+      | EvictBM_SK s _ s' _ t, Spec.EvictBM k k' t' ->  
+          lemma_vevictbm_simulates_spec vs vs' s s' k k' t
+    else
+      match e with
+      | Get_SK s _ v -> lemma_vget_has_failed vs s v
+      | Put_SK s _ v -> lemma_vput_has_failed vs s v
+      | AddM_SK s r s' _ -> lemma_vaddm_has_failed vs s s' r
+      | EvictM_SK s _ s' _ -> lemma_vevictm_has_failed vs s s'
+      | AddB_SK s r t j -> lemma_vaddb_has_failed vs s r t j
+      | EvictB_SK s _ t -> lemma_vevictb_has_failed vs s t
+      | EvictBM_SK s _ s' _ t -> lemma_vevictbm_has_failed vs s s' t
+
+let rec lemma_t_verify_aux_simulates_spec (vs:vtls) (vs':Spec.vtls) (l:logSK) (l':logK)
+  : Lemma (requires (vtls_rel vs vs' /\ Seq.length l = Seq.length l' /\ (Valid? vs ==> log_rel_with_vtls vs l l')))
+          (ensures (vtls_rel (t_verify_aux vs l) (Spec.t_verify_aux vs' l')))
+          (decreases (Seq.length l))
+  = let n = Seq.length l in
+    if n <> 0
+    then
+      (* intermediate repr. *)
+      let l2 = prefix l (n - 1) in
+      let vs2 = t_verify_aux vs l2 in
+      let e = Seq.index l (n - 1) in
+      (* spec repr. *)
+      let l2' = prefix l' (n - 1) in
+      let vs2' = Spec.t_verify_aux vs' l2' in
+      let e' = Seq.index l' (n - 1) in
+      if Valid? vs 
+      then (
+        lemma_t_verify_aux_simulates_spec vs vs' l2 l2';
+        lemma_t_verify_step_simulates_spec vs2 vs2' e e' 
+      )
+      else admit() // in this case, both results are Failed
+
 let lemma_t_verify_simulates_spec (id:thread_id) (l:logSK) (l':logK)
   : Lemma (requires (log_rel l l'))
           (ensures (vtls_rel (t_verify id l) (Spec.t_verify id l')))
-  = 
-
-(* For any log, the intermediate implementation will verify 
-   iff the the spec implementation does. *)
-
-let lemma_verifiable_simulates_spec (id:thread_id) (l:logSK) (l':logK)
-  : Lemma (requires (log_rel l l'))
-          (ensures (let tl : VT.thread_id_vlog = (id,l') in
-                    verifiable id l = VT.verifiable tl))
-  = lemma_t_verify_simulates_spec id l l';
-    let vs = t_verify id l in
-    if Valid? vs
-    then if not (thread_store_is_map vs) 
-    then admit()
-*)
+  = lemma_init_thread_state_rel id;
+    lemma_log_rel l l';
+    lemma_t_verify_aux_simulates_spec (init_thread_state id) (Spec.init_thread_state id) l l'
