intermediate/Veritas.Intermediate.VerifySKC.fsti
@@ -83,6 +83,121 @@ val vevictb (s:slot_id) (t:timestamp) (vs:vtls {Valid? vs}): vtls
 
 val vevictbm (s:slot_id) (s':slot_id) (t:timestamp) (vs:vtls {Valid? vs}): vtls
 
+(* Relation between stores *)
+let store_rel (st:vstore) (st':Spec.vstore) : Type = 
+  st.is_map /\ FE.feq st' (as_map st)
+
+(* Relation between thread-local states *)
+let has_failed (vs:vtls) = Failed? vs || not (thread_store_is_map vs)
+let vtls_rel (vs:vtls) (vs':Spec.vtls) : Type =
+  if has_failed vs then Spec.Failed? vs'
+  else 
+    match vs, vs' with
+    | Valid id st clk ha he, Spec.Valid id' st' clk' _ ha' he' ->
+        store_rel st st' /\ 
+        // other fields related by equality  
+        id = id' /\ clk = clk' /\ ha = ha' /\ he = he'   
+    | _, _ -> False
+
+(* Relation between a slot and key *)
+let slot_key_rel (vs: vtls {Valid? vs}) (s:slot_id) (k:key) =
+  let st = thread_store vs in slot_key_equiv st s k
+
+(* Simulation lemmas for v* functions *)
+
+val lemma_vget_simulates_spec 
+      (vs:vtls{Valid? vs})
+      (vs':Spec.vtls{Spec.Valid? vs'})
+      (s:slot_id)
+      (k:data_key)
+      (v:data_value)
+  : Lemma (requires (vtls_rel vs vs' /\ slot_key_rel vs s k))
+          (ensures (vtls_rel (vget s v vs) (Spec.vget k v vs')))
+
+val lemma_vget_has_failed (vs:vtls{Valid? vs}) (s:slot_id) (v:data_value)
+  : Lemma (requires (not (thread_store_is_map vs)))
+          (ensures (has_failed (vget s v vs)))
+
+val lemma_vput_simulates_spec 
+      (vs:vtls{Valid? vs}) 
+      (vs':Spec.vtls{Spec.Valid? vs'}) 
+      (s:slot_id) 
+      (k:data_key) 
+      (v:data_value) 
+  : Lemma (requires (vtls_rel vs vs' /\ slot_key_rel vs s k))
+          (ensures (vtls_rel (vput s v vs) (Spec.vput k v vs'))) 
+
+val lemma_vput_has_failed (vs:vtls{Valid? vs}) (s:slot_id) (v:data_value)
+  : Lemma (requires (not (thread_store_is_map vs)))
+          (ensures (has_failed (vput s v vs)))
+
+val lemma_vaddm_simulates_spec 
+      (vs:vtls{Valid? vs}) 
+      (vs':Spec.vtls{Spec.Valid? vs'}) 
+      (s s':slot_id)
+      (r:record)
+      (k':merkle_key)  
+  : Lemma (requires (vtls_rel vs vs') /\ slot_key_rel vs s' k')
+          (ensures (vtls_rel (vaddm s r s' vs) (Spec.vaddm r k' vs'))) 
+
+val lemma_vaddm_has_failed (vs:vtls{Valid? vs}) (s s':slot_id) (r:record)
+  : Lemma (requires (not (thread_store_is_map vs)))
+          (ensures (has_failed (vaddm s r s' vs)))
+
+val lemma_vevictm_simulates_spec 
+      (vs:vtls{Valid? vs}) 
+      (vs':Spec.vtls{Spec.Valid? vs'}) 
+      (s s':slot_id)
+      (k:key)
+      (k':merkle_key)  
+  : Lemma (requires (vtls_rel vs vs' /\ slot_key_rel vs s k /\ slot_key_rel vs s' k'))
+          (ensures (vtls_rel (vevictm s s' vs) (Spec.vevictm k k' vs'))) 
+
+val lemma_vevictm_has_failed (vs:vtls{Valid? vs}) (s s':slot_id)
+  : Lemma (requires (not (thread_store_is_map vs)))
+          (ensures (has_failed (vevictm s s' vs)))
+
+val lemma_vaddb_simulates_spec 
+      (vs:vtls{Valid? vs}) 
+      (vs':Spec.vtls{Spec.Valid? vs'}) 
+      (s:slot_id)
+      (r:record)
+      (t:timestamp)
+      (j:thread_id)
+  : Lemma (requires (vtls_rel vs vs'))
+          (ensures (vtls_rel (vaddb s r t j vs) (Spec.vaddb r t j vs')))
+
+val lemma_vaddb_has_failed (vs:vtls{Valid? vs}) (s:slot_id) (r:record) (t:timestamp) (j:thread_id)
+  : Lemma (requires (not (thread_store_is_map vs)))
+          (ensures (has_failed (vaddb s r t j vs)))
+
+val lemma_vevictb_simulates_spec 
+      (vs:vtls{Valid? vs}) 
+      (vs':Spec.vtls{Spec.Valid? vs'}) 
+      (s:slot_id)
+      (k:key)
+      (t:timestamp)
+  : Lemma (requires (vtls_rel vs vs' /\ slot_key_rel vs s k))
+          (ensures (vtls_rel (vevictb s t vs) (Spec.vevictb k t vs'))) 
+
+val lemma_vevictb_has_failed (vs:vtls{Valid? vs}) (s:slot_id) (t:timestamp)
+  : Lemma (requires (not (thread_store_is_map vs)))
+          (ensures (has_failed (vevictb s t vs)))
+
+val lemma_vevictbm_simulates_spec 
+      (vs:vtls{Valid? vs}) 
+      (vs':Spec.vtls{Spec.Valid? vs'}) 
+      (s s':slot_id)
+      (k:key)
+      (k':merkle_key)
+      (t:timestamp)
+  : Lemma (requires (vtls_rel vs vs' /\ slot_key_rel vs s k /\ slot_key_rel vs s' k'))
+          (ensures (vtls_rel (vevictbm s s' t vs) (Spec.vevictbm k k' t vs'))) 
+
+val lemma_vevictbm_has_failed (vs:vtls{Valid? vs}) (s s':slot_id) (t:timestamp)
+  : Lemma (requires (not (thread_store_is_map vs)))
+          (ensures (has_failed (vevictbm s s' t vs)))
+
 (* Note that the key values aren't used in the v* functions -
    they are just useful (maybe?) for proof *)
 let t_verify_step (vs:vtls) (e:logSK_entry): vtls =
@@ -111,7 +226,6 @@ let rec t_verify_aux (vs:vtls) (l:logSK): Tot vtls
 
 (* Main verify function *)
 val init_thread_state (id:thread_id): vtls
-
 let t_verify (id:thread_id) (l:logSK): vtls = 
   t_verify_aux (init_thread_state id) l 
 
@@ -124,108 +238,44 @@ let verify (id:thread_id) (l:logSK): vtls =
 let verifiable (id:thread_id) (l: logSK): bool =
   Valid? (verify id l)
 
-(* Relation between stores *)
-let store_rel (st:vstore) (st':Spec.vstore) : Type = 
-  st.is_map /\ FE.feq st' (as_map st)
+val init_thread_state_valid (id:thread_id)
+  : Lemma (Valid? (init_thread_state id))
+          [SMTPat (init_thread_state id)]
 
-(* Relation between thread-local states *)
-let vtls_rel (vs:vtls) (vs':Spec.vtls) : Type =
-  match vs, vs' with
-  // either both runs failed
-  | Failed, Spec.Failed -> True
-  // or both are valid and the stores are related
-  | Valid id st clk ha he, Spec.Valid id' st' clk' _ ha' he' ->
-       store_rel st st' /\ 
-       // other fields related by equality  
-       id = id' /\ clk = clk' /\ ha = ha' /\ he = he'   
-  // or the spec run failed, but the store of vs is not a map
-  | Valid _ st _ _ _, _ -> not st.is_map
-  | _, _ -> False
-
-(* Relation between a slot and key *)
-let slot_key_rel (vs: vtls {Valid? vs}) (s:slot_id) (k:key) =
-  let st = thread_store vs in slot_key_equiv st s k
-
-val lemma_vget_simulates_spec 
-      (vs:vtls{Valid? vs})
-      (vs':Spec.vtls{Spec.Valid? vs'})
-      (s:slot_id)
-      (k:data_key)
-      (v:data_value)
-  : Lemma (requires (vtls_rel vs vs' /\ slot_key_rel vs s k))
-          (ensures (vtls_rel (vget s v vs) (Spec.vget k v vs')))
-
-val lemma_vput_simulates_spec 
-      (vs:vtls{Valid? vs}) 
-      (vs':Spec.vtls{Spec.Valid? vs'}) 
-      (s:slot_id) 
-      (k:data_key) 
-      (v:data_value) 
-  : Lemma (requires (vtls_rel vs vs' /\ slot_key_rel vs s k))
-          (ensures (vtls_rel (vput s v vs) (Spec.vput k v vs'))) 
-
-val lemma_vaddm_simulates_spec 
-      (vs:vtls{Valid? vs}) 
-      (vs':Spec.vtls{Spec.Valid? vs'}) 
-      (s s':slot_id)
-      (r:record)
-      (k':merkle_key)  
-  : Lemma (requires (vtls_rel vs vs') /\ slot_key_rel vs s' k')
-          (ensures (vtls_rel (vaddm s r s' vs) (Spec.vaddm r k' vs'))) 
-
-val lemma_vevictm_simulates_spec 
-      (vs:vtls{Valid? vs}) 
-      (vs':Spec.vtls{Spec.Valid? vs'}) 
-      (s s':slot_id)
-      (k:key)
-      (k':merkle_key)  
-  : Lemma (requires (vtls_rel vs vs' /\ slot_key_rel vs s k /\ slot_key_rel vs s' k'))
-          (ensures (vtls_rel (vevictm s s' vs) (Spec.vevictm k k' vs'))) 
-
-val lemma_vaddb_simulates_spec 
-      (vs:vtls{Valid? vs}) 
-      (vs':Spec.vtls{Spec.Valid? vs'}) 
-      (s:slot_id)
-      (r:record)
-      (t:timestamp)
-      (j:thread_id)
-  : Lemma (requires (vtls_rel vs vs'))
-          (ensures (vtls_rel (vaddb s r t j vs) (Spec.vaddb r t j vs')))
-
-val lemma_vevictb_simulates_spec 
-      (vs:vtls{Valid? vs}) 
-      (vs':Spec.vtls{Spec.Valid? vs'}) 
-      (s:slot_id)
-      (k:key)
-      (t:timestamp)
-  : Lemma (requires (vtls_rel vs vs' /\ slot_key_rel vs s k))
-          (ensures (vtls_rel (vevictb s t vs) (Spec.vevictb k t vs'))) 
-
-val lemma_vevictbm_simulates_spec 
-      (vs:vtls{Valid? vs}) 
-      (vs':Spec.vtls{Spec.Valid? vs'}) 
-      (s s':slot_id)
-      (k:key)
-      (k':merkle_key)
-      (t:timestamp)
-  : Lemma (requires (vtls_rel vs vs' /\ slot_key_rel vs s k /\ slot_key_rel vs s' k'))
-          (ensures (vtls_rel (vevictbm s s' t vs) (Spec.vevictbm k k' t vs'))) 
+val lemma_init_thread_state_rel (id:thread_id) :
+  Lemma (vtls_rel (init_thread_state id) (Spec.init_thread_state id))
 
 (* Relation between logs -- haven't really worked this out yet *)
 let log_rel  (l:logSK) (l':logK) : Type 
   = skc l /\ drop_slots l = l'
 
-// The property we want for log_rel:
-//   * l and l' have matching entries, and their keys & slots are related given 
-//     the state computed so far
+// whatever the defn of log_rel, it should satisfy lemma_log_rel
+let log_entry_rel (vs:vtls{Valid? vs}) (e:logSK_entry) (e':logK_entry) : Type
+  = match e, e' with
+    | Get_SK s _ v, Spec.Get k v' -> slot_key_rel vs s k /\ v = v'
+    | Put_SK s _ v, Spec.Put k v' -> slot_key_rel vs s k /\ v = v'
+    | AddM_SK s r s' _, Spec.AddM r' k' -> r = r' /\ slot_key_rel vs s' k'
+    | EvictM_SK s _ s' _, Spec.EvictM k k' -> slot_key_rel vs s k /\ slot_key_rel vs s' k'
+    | AddB_SK s r t j, Spec.AddB r' t' j' -> r = r' /\ t = t' /\ j = j' 
+    | EvictB_SK s _ t, Spec.EvictB k t' -> slot_key_rel vs s k /\ t = t'
+    | EvictBM_SK s _ s' _ t, Spec.EvictBM k k' t' -> slot_key_rel vs s k /\ slot_key_rel vs s' k' /\ t = t'
+    | _, _ -> False
 
-val lemma_init_thread_state_rel (id:thread_id) :
-  Lemma (vtls_rel (init_thread_state id) (Spec.init_thread_state id))
+let log_rel_with_vtls (vs:vtls{Valid? vs}) (l:logSK) (l':logK) : Type 
+  = Seq.length l = Seq.length l' /\
+    (forall (i:seq_index l). 
+       let vs2 = t_verify_aux vs (prefix l i) in
+       Valid? vs2 ==>
+       log_entry_rel vs2 (Seq.index l i) (Seq.index l' i))
 
-let lemma_t_verify_simulates_spec (id:thread_id) (l:logSK) (l':logK)
+let lemma_log_rel (l:logSK) (l':logK) 
+  : Lemma (requires (log_rel l l'))
+          (ensures (forall (id:thread_id). log_rel_with_vtls (init_thread_state id) l l')) 
+  = admit()
+
+val lemma_t_verify_simulates_spec (id:thread_id) (l:logSK) (l':logK)
   : Lemma (requires (log_rel l l'))
           (ensures (vtls_rel (t_verify id l) (Spec.t_verify id l')))
-  = admit()
 
 (* For any log, the intermediate implementation will verify 
    iff the the spec implementation does. *)
